- ((652f3d0a-9912-44ed-9451-599e31a37b19))
- collapsed:: true
  $$\Delta x=\frac{(v_f+v_i)t}{2}$$
	- this works because the shape below the line is a trapezoid
	  collapsed:: true
		- the smaller base of the trapezoid is $$v_i$$, and the bigger base is $$v_f$$
		-
	- the equation is essentially the area of a trapezoid
- collapsed:: true
  $$v_f=v_i+at$$
	- this equation uses the properties of $$a$$, where $$a$$ is the acceleration of object/slope of the graph
	- since $$slope=\dfrac{\Delta y}{\Delta x}$$, then $$slope\: \cdot\: \Delta x = \Delta y$$, rewritten as $$at = \Delta v$$
- collapsed:: true
  $$x_f=x_i+v_it+\dfrac{at^2}{2}$$
	- each of these terms do different to essentially build the trapezoid as mentioned in
	   [{{embed ((64ea470a-6ca6-4f10-8459-48b500a9c8c8))}}](logseq://graph/notes?block-id=64ea470a-6ca6-4f10-8459-48b500a9c8c8)
	- the trapezoid can be split into two parts, a square and a triangle
	- the square is calculated by $$v_i$$
	- the triangle is calculated by taking half of multiplying $$t$$ with the difference of $$v_i $$ and $$ v_f$$, or $$at$$, giving us $$\dfrac{at^2}{2}$$,
	  collapsed:: true
		- {{embed ((64ea470a-3314-4a3b-8f40-060a174076df))}}
	- the $$x_i$$ can be taken out if not necessary, as it only adds previous displacement
- collapsed:: true
  $$v^2_f=v^2_i+2a\Delta x$$
	- the $$\Delta x$$ can be changed to $$t^2$$ or $$(x-x_0)$$ or just $$s$$
	- this works by forming a square with the side length of $$v_f$$
	- the reason behind $$2a\Delta x$$ is because by multiplying the trapezoids by a, we get a trapezoid with the height equaling to the difference of $$v_i$$ and $$v_f$$
	- the equaling height and difference creates a trapezoid with a slope of 1, which allows it to be multiplied by two, forming the square of $$v_f$$
	- if $$a$$ is positive, it adds towards $$v_i$$, if $$a$$ is negative, it subtracts from $$v_i$$,
- $$v_{avg}=\dfrac{\Delta x}{\Delta t}$$
- {{embed ((652ff1bf-9dd5-4f69-9e02-9528a7a9d070))}}
- $$f_{spring}=-kx$$
- ((652816f3-7a17-46c0-844b-5571b67cd789))
- collapsed:: true
  $$T=\dfrac{1}{f}$$
	- $$f=\dfrac{1}{T}$$
- collapsed:: true
  $$a_c=\dfrac{V_T^2}{r^2}$$
	- $$a_c\cdot r^2=V_T^2$$
	- $$r=\sqrt{\dfrac{V_T^2}{a_c}}$$
- collapsed:: true
  $$V_t=\dfrac{(c)/ (2\pi r)}{T}$$
	- $$T=\dfrac{2\pi r}{V_t}$$
-